ironfleet/src/Dafny/Distributed/Protocol/RSL/PerformanceProof/Phase2Proof.i.dfy
@@ -34,11 +34,11 @@ predicate RslAssumption(s:TimestampedRslState)
   && |s.t_replicas| > 0
   && s.constants.params.max_batch_size == 1
 
-  // TODO: Remove this assumption
   && (var nextStep := s.t_environment.nextStep; nextStep.LEnvStepHostIos? ==>
   (forall io :: io in nextStep.ios && io.LIoOpReceive? ==> !io.r.msg.v.RslMessage_Heartbeat?))
   && LeaderAlwaysZero(s)
-  && SelfDelivery < D
+  && minD < SelfDelivery < D < 2*minD
+  && ProcessPacket > 0
 }
 
 predicate RslConsistency(s:TimestampedRslState)
@@ -47,12 +47,43 @@ predicate RslConsistency(s:TimestampedRslState)
     && WellFormedLConfiguration(s.constants.config)
 }
 
+predicate ServersAreNotClients(s:TimestampedRslState)
+{
+  forall id :: id in s.constants.config.clientIds && id in s.constants.config.replica_ids
+    ==> false
+}
+
+predicate RequestBatchServersAreNotClients(s:TimestampedRslState, v:RequestBatch)
+{
+  forall r :: r in v ==> r.client in s.constants.config.clientIds
+}
+
 predicate AlwaysInvariant(s:TimestampedRslState)
 {
   && (forall pkt :: pkt in s.undeliveredPackets ==>
-    pkt in s.t_environment.sentPackets
+    && pkt in s.t_environment.sentPackets
     && pkt.src in s.constants.config.replica_ids
-    && pkt.dst in s.constants.config.replica_ids)
+    && pkt.dst in s.constants.config.replica_ids
+  )
+
+  && ServersAreNotClients(s)
+
+  && (forall pkt :: pkt in s.undeliveredPackets ==>
+    && (pkt.msg.v.RslMessage_2a? ==> RequestBatchServersAreNotClients(s, pkt.msg.v.val_2a))
+    && (pkt.msg.v.RslMessage_2b? ==> RequestBatchServersAreNotClients(s, pkt.msg.v.val_2b))
+  )
+
+  && (forall idx :: 0 <= idx < |s.t_replicas|
+  ==>
+  && (var uls := s.t_replicas[idx].v.replica.learner.unexecuted_learner_state;
+   forall opn :: opn in uls ==> RequestBatchServersAreNotClients(s, uls[opn].candidate_learned_value)
+  )
+
+  && (s.t_replicas[idx].v.replica.executor.next_op_to_execute.OutstandingOpKnown?
+  ==> RequestBatchServersAreNotClients(s, s.t_replicas[idx].v.replica.executor.next_op_to_execute.v)
+  )
+
+  )
 }
 
 predicate LSchedulerLagTimeBound(tls:TimestampedLScheduler)
@@ -76,6 +107,20 @@ predicate LeaderNextOperationNumberInvariant(s:LProposer, log_truncation_point:O
     && |s.received_1b_packets| >= LMinQuorumSize(s.constants.all.config)
 
     && LtUpperBound(s.next_operation_number_to_propose, s.constants.all.params.max_integer_val)
+}
+
+predicate ProposedLeaderNextOperationNumberInvariant(s:LProposer, log_truncation_point:OperationNumber)
+{
+  && LSetOfMessage1bAboutBallot(s.received_1b_packets, s.max_ballot_i_sent_1a)
+
+    && 0 < s.next_operation_number_to_propose <= UpperBoundedAddition(log_truncation_point, s.constants.all.params.max_log_length, s.constants.all.params.max_integer_val)
+
+    && (forall pkt :: pkt in s.received_1b_packets
+    ==>
+    && pkt.msg.log_truncation_point == 0
+    && pkt.msg.votes == map[]
+    )
+    && |s.received_1b_packets| >= LMinQuorumSize(s.constants.all.config)
 }
 
 predicate Pre2aInvariant(s:TimestampedRslState, req_time:Timestamp)
@@ -110,62 +155,124 @@ predicate Pre2aInvariant(s:TimestampedRslState, req_time:Timestamp)
   && |s.undeliveredPackets| == 0
 }
 
-datatype Phase2Progress = P2a(/*pkt:TimestampedRslPacket*/) | P2b | P2done
-
-predicate GenericPhase2UndeliveredPacketInvariant(undeliveredPackets:UndeliveredPackets, req_time:Timestamp, progresses:map<NodeIdentity, Phase2Progress>)
+predicate No2aToDst(undeliveredPackets:UndeliveredPackets, dst:NodeIdentity)
 {
   && (forall pkt :: pkt in undeliveredPackets
+    && pkt.msg.v.RslMessage_2a?
+    ==> pkt.dst != dst)
+}
+
+predicate No2bToLeaderFromSrc(undeliveredPackets:UndeliveredPackets, ldr:NodeIdentity, dst:NodeIdentity)
+{
+  && (forall pkt :: pkt in undeliveredPackets
+    && pkt.msg.v.RslMessage_2a?
+    ==> pkt.dst != dst)
+}
+
+datatype Phase2Progress = P2a(pkt:TimestampedRslPacket) | P2b | P2done
+
+predicate GenericPhase2UndeliveredPacketInvariant(undeliveredPackets:UndeliveredPackets, constants:LConstants, req_time:Timestamp, t2a:Timestamp, progresses:map<NodeIdentity, Phase2Progress>)
+  requires 0 < |constants.config.replica_ids|
+{
+  && (forall pkt :: pkt in undeliveredPackets && pkt.dst in constants.config.replica_ids
   ==>
   pkt.msg.v.RslMessage_2a?
   || pkt.msg.v.RslMessage_2b?
   )
 
-  && (forall pkt :: pkt in undeliveredPackets && pkt.msg.v.RslMessage_2a?
-      ==> pkt.dst in progresses && progresses[pkt.dst] == P2a()
+  && (forall pkt {:trigger pkt.msg.v.RslMessage_2a?} :: pkt in undeliveredPackets && pkt.msg.v.RslMessage_2a?
+      ==> pkt.dst in progresses && progresses[pkt.dst].P2a?
       && TimeLe(pkt.msg.ts, TimeBound2aDelivery(req_time))
+      && t2a + minD < pkt.msg.ts <= t2a + D
+      && (var undeliveredPackets' := undeliveredPackets - {pkt};
+      No2aToDst(undeliveredPackets', pkt.dst)
+      )
   )
 
-  && (forall pkt :: pkt in undeliveredPackets && pkt.msg.v.RslMessage_2b?
+  && (forall pkt {:trigger pkt.msg.v.RslMessage_2b?} :: pkt in undeliveredPackets && pkt.msg.v.RslMessage_2b?
       ==> pkt.src in progresses && progresses[pkt.src] == P2b
-      && TimeLe(pkt.msg.ts, TimeBound2bDelivery(req_time))
+      && pkt.msg.ts > t2a + 2*minD
+      // && TimeLe(pkt.msg.ts, TimeBound2bDelivery(req_time))
+
+      // && (var undeliveredPackets' := undeliveredPackets - {pkt};
+      // No2bToLeaderFromSrc(undeliveredPackets', constants.config.replica_ids[0], pkt.src)
+      // )
+  )
+
+  && (forall id {:trigger id in progresses} ::
+    Progress2aProperty(progresses, id, undeliveredPackets) 
   )
 }
+
+predicate {:opaque} Progress2aProperty(progresses:map<NodeIdentity,Phase2Progress>, id:NodeIdentity, undeliveredPackets:UndeliveredPackets)
+{
+  id in progresses && progresses[id].P2a?
+    ==>
+    progresses[id].pkt in undeliveredPackets
+    && progresses[id].pkt.msg.v.RslMessage_2a?
+    && progresses[id].pkt.dst == id
+}
+
+lemma SelectiveProgress2aProperty(progresses:map<NodeIdentity,Phase2Progress>, id:NodeIdentity, undeliveredPackets:UndeliveredPackets)
+  ensures Progress2aProperty(progresses, id, undeliveredPackets) <==> (id in progresses && progresses[id].P2a? ==> progresses[id].pkt in undeliveredPackets && progresses[id].pkt.msg.v.RslMessage_2a? && progresses[id].pkt.dst == id)
+{
+  reveal_Progress2aProperty(); 
+}
   
-predicate GenericPhase2Invariant(s:TimestampedRslState, req_time:Timestamp, progresses:map<NodeIdentity, Phase2Progress>)
+predicate GenericPhase2Invariant(s:TimestampedRslState, req_time:Timestamp, t2a:Timestamp, progresses:map<NodeIdentity, Phase2Progress>)
   requires RslConsistency(s)
 {
   && (forall id :: id in progresses.Keys <==> id in s.constants.config.replica_ids)
   && (0 < |s.t_replicas|
     ==>
     |s.t_replicas[0].v.replica.proposer.request_queue| == 0
-    // && LSchedulerLagTimeBound(s.t_replicas[0])
-    // && TimeLe(s.t_replicas[0].dts, req_time)
-  )
 
-  && GenericPhase2UndeliveredPacketInvariant(s.undeliveredPackets, req_time, progresses)
+    && GenericPhase2UndeliveredPacketInvariant(s.undeliveredPackets, s.constants, req_time, t2a, progresses)
+  )
 
   && (forall idx :: && 0 < idx < |s.t_replicas|
   ==>
-  (progresses[s.constants.config.replica_ids[idx]].P2a?
-    ==> LSchedulerLagTimeBound(s.t_replicas[idx]))
+  // && s.t_replicas[idx].v.replica.executor.next_op_to_execute == OutstandingOpUnknown()
+  && (progresses[s.constants.config.replica_ids[idx]].P2a?
+      ==> LSchedulerLagTimeBound(s.t_replicas[idx])
+        && s.t_replicas[idx].v.replica.learner.unexecuted_learner_state == map[]
+   )
   )
 }
 
-predicate Phase2UnacceptedLeaderInvariant(s:TimestampedRslState, req_time:Timestamp, progresses:map<NodeIdentity, Phase2Progress>)
+predicate Phase2UnacceptedLeaderInvariant(s:TimestampedRslState, req_time:Timestamp, t2a:Timestamp, progresses:map<NodeIdentity, Phase2Progress>)
   requires RslConsistency(s)
 {
-  && GenericPhase2Invariant(s, req_time, progresses)
+  && GenericPhase2Invariant(s, req_time, t2a, progresses)
 
   && (0 < |s.t_replicas|
     ==>
     |s.t_replicas[0].v.replica.proposer.request_queue| == 0
     && 0 <= s.t_replicas[0].v.nextActionIndex < 10
     && TimeLe(s.t_replicas[0].ts, s.t_replicas[0].dts + TimeActionRange(0) + TimeActionRange(s.t_replicas[0].v.nextActionIndex))
+    && progresses[s.constants.config.replica_ids[0]].P2a?
+    && s.t_replicas[0].v.replica.learner.unexecuted_learner_state == map[]
+    && s.t_replicas[0].v.replica.executor.next_op_to_execute == OutstandingOpUnknown()
+    && ProposedLeaderNextOperationNumberInvariant(s.t_replicas[0].v.replica.proposer, s.t_replicas[0].v.replica.acceptor.log_truncation_point)
+  )
+}
+
+predicate Phase2AcceptedLeaderInvariant(s:TimestampedRslState, req_time:Timestamp, t2a:Timestamp, progresses:map<NodeIdentity, Phase2Progress>)
+  requires RslConsistency(s)
+{
+  && GenericPhase2Invariant(s, req_time, t2a, progresses)
+
+  && (0 < |s.t_replicas|
+    ==>
+    |s.t_replicas[0].v.replica.proposer.request_queue| == 0
+    && 0 <= s.t_replicas[0].v.nextActionIndex < 10
+    // && TimeLe(s.t_replicas[0].ts, s.t_replicas[0].dts + TimeActionRange(0) + TimeActionRange(s.t_replicas[0].v.nextActionIndex))
+    && !progresses[s.constants.config.replica_ids[0]].P2a?
   )
 }
 
 lemma lemma_leader_3_Pre2aGoesToPhase2UnacceptedLeader(s:TimestampedRslState, s':TimestampedRslState, j:int, req_time:Timestamp) returns
-  (progresses':map<NodeIdentity,Phase2Progress>)
+  (progresses':map<NodeIdentity,Phase2Progress>, t2a:Timestamp)
   requires RslAssumption(s);
   requires RslAssumption(s');
   requires RslConsistency(s);
@@ -181,15 +288,200 @@ lemma lemma_leader_3_Pre2aGoesToPhase2UnacceptedLeader(s:TimestampedRslState, s'
   requires TimestampedRslNextOneReplica(s, s', j, s.t_environment.nextStep.ios);
 
   requires Pre2aInvariant(s, req_time)
-  ensures Phase2UnacceptedLeaderInvariant(s', req_time, progresses')
+  ensures Phase2UnacceptedLeaderInvariant(s', req_time, t2a, progresses')
 {
+  reveal_Progress2aProperty();
   var t_ios := s.t_environment.nextStep.ios;
-  progresses' := map id | id in s.constants.config.replica_ids :: P2a; // (var pkt :| LIoOpSend(pkt) in t_ios; P2a(pkt)) ;
+  var ios := UntagLIoOpSeq(t_ios);
+  var sent_packets := ExtractSentPacketsFromIos(ios);
+
+  // assert exists pkt :: LIoOpSend(pkt) in t_ios;
+  // assert exists pkt:TimestampedRslPacket :: pkt.msg.v.RslMessage_2a? && pkt.dst == s.constants.config.replica_ids[j] && LIoOpSend(pkt) in t_ios;
+
+  var i := 0;
+  progresses' := map[];
+  
+  while i < |s.constants.config.replica_ids|
+    invariant 0 <= i <= |s.constants.config.replica_ids|;
+    invariant (forall id :: id in progresses'.Keys <==> id in s.constants.config.replica_ids[..i]);
+    invariant (forall id :: id in progresses'
+      ==>
+      && progresses'[id].P2a? && progresses'[id].pkt in s'.undeliveredPackets
+      && progresses'[id].pkt.msg.v.RslMessage_2a? && progresses'[id].pkt.dst == id
+    );
+  {
+    var untagged_pkt := sent_packets[i];
+    var j:int :| 0 <= j < |ios| && ios[j] == LIoOpSend(sent_packets[i]);
+    var pkt := t_ios[j].s;
+
+    progresses' := progresses'[s.constants.config.replica_ids[i] := P2a(pkt)];
+    i := i + 1;
+  }
+  t2a := s'.t_replicas[0].ts;
 }
 
-lemma lemma_notleader_any_P2UnacceptedGoesToP2Unaccepted(s:TimestampedRslState, s':TimestampedRslState, j:int, req_time:Timestamp)
+lemma lemma_notleader_notreceive_P2UnacceptedGoesToP2Unaccepted(s:TimestampedRslState, s':TimestampedRslState, j:int, req_time:Timestamp, t2a:Timestamp, progresses:map<NodeIdentity, Phase2Progress>)
   returns (progresses':map<NodeIdentity,Phase2Progress>)
+
+  requires RslAssumption(s);
+  requires RslAssumption(s');
+  requires RslConsistency(s);
+  requires RslConsistency(s');
+  requires 0 <= j < |s.constants.config.replica_ids|;
+
+  requires j > 0;
+
+  requires s.t_environment.nextStep.LEnvStepHostIos?;
+  requires s.t_environment.nextStep.actor == s.constants.config.replica_ids[j];
+  requires s.t_environment.nextStep.nodeStep != RslStep(0);
+  requires s.t_environment.nextStep.nodeStep == RslStep(6);
+
+  requires TimestampedRslNextOneReplica(s, s', j, s.t_environment.nextStep.ios);
+
+  requires Phase2UnacceptedLeaderInvariant(s, req_time, t2a, progresses)
+  ensures Phase2UnacceptedLeaderInvariant(s', req_time, t2a, progresses')
 {
+  reveal_Progress2aProperty();
+  progresses' := progresses;
+  var t_ios := s.t_environment.nextStep.ios;
+  var sent_packets := ExtractSentPacketsFromIos(UntagLIoOpSeq(t_ios));
+
+  if (LExecutorExecute.requires(s.t_replicas[j].v.replica.executor, s'.t_replicas[j].v.replica.executor, sent_packets)
+  && LExecutorExecute(s.t_replicas[j].v.replica.executor, s'.t_replicas[j].v.replica.executor, sent_packets)) {
+    var e := s.t_replicas[j].v.replica.executor;
+    var e' := s'.t_replicas[j].v.replica.executor;
+    var batch := e.next_op_to_execute.v;
+    var temp := HandleRequestBatch(e.app, batch);
+    var new_state := temp.0[|temp.0|-1];
+    var replies := temp.1;
+
+    assert sent_packets == GetPacketsFromReplies(e.constants.all.config.replica_ids[e.constants.my_index], batch, replies);
+
+    forall i |
+      0 <= i < |sent_packets|
+
+      ensures sent_packets[i].dst in s.constants.config.clientIds
+      ensures sent_packets[i].dst !in s.constants.config.replica_ids
+    {
+      lemma_SizeOfGetPacketsFromReplies(s.constants.config.replica_ids[j], batch, replies, sent_packets);
+      lemma_SpecificPacketInGetPacketsFromReplies(s.constants.config.replica_ids[j], batch, replies, sent_packets, i);
+      assert sent_packets[i].dst == batch[i].client;
+      assert batch[i].client in s.constants.config.clientIds;
+    }
+  } else {
+  }
+}
+
+lemma lemma_notleader_receive_P2UnacceptedGoesToP2Unaccepted(s:TimestampedRslState, s':TimestampedRslState, j:int, req_time:Timestamp, t2a:Timestamp, progresses:map<NodeIdentity, Phase2Progress>)
+  returns (progresses':map<NodeIdentity,Phase2Progress>)
+
+  requires RslAssumption(s);
+  requires RslAssumption(s');
+  requires RslConsistency(s);
+  requires RslConsistency(s');
+  requires 0 <= j < |s.constants.config.replica_ids|;
+
+  requires j > 0;
+
+  requires s.t_environment.nextStep.LEnvStepHostIos?;
+  requires s.t_environment.nextStep.actor == s.constants.config.replica_ids[j];
+  requires s.t_environment.nextStep.nodeStep == RslStep(0);
+
+  requires TimestampedRslNextOneReplica(s, s', j, s.t_environment.nextStep.ios);
+
+  requires Phase2UnacceptedLeaderInvariant(s, req_time, t2a, progresses)
+  ensures Phase2UnacceptedLeaderInvariant(s', req_time, t2a, progresses')
+{
+  reveal_PacketDeliveredInOrder();
+  reveal_Progress2aProperty();
+
+  progresses' := progresses;
+
+  var ios := s.t_environment.nextStep.ios;
+  assert ReplicasDistinct(s.constants.config.replica_ids, 0, j);
+  progresses' := progresses;
+  SelectiveProgress2aProperty(progresses, s.constants.config.replica_ids[j], s.undeliveredPackets);
+  if !progresses[s.constants.config.replica_ids[j]].P2a? {
+    progresses' := progresses;
+  }
+  else {
+    if ios[0].LIoOpReceive? {
+      var pkt_2a := progresses[s.constants.config.replica_ids[j]].pkt;
+
+      if ios[0].r.msg.v.RslMessage_2b? {
+        assert ios[0].r.msg.ts <= pkt_2a.msg.ts;
+        assert pkt_2a.msg.ts < t2a + D;
+        assert t2a + 2*minD < ios[0].r.msg.ts;
+        assert false;
+      }
+
+      assert (ios[0].r.msg.v.RslMessage_2a?);
+      BoundedLagImpliesBoundedProcessingTime(s.t_replicas[j].dts, s.t_replicas[j].ts, ios[0].r.msg.ts, s'.t_replicas[j].ts, TimeActionRange(0));
+      progresses' := progresses[s.constants.config.replica_ids[j] := P2b];
+
+     // assert (forall io :: io in ios && io.LIoOpSend? && io.s.msg.v.RslMessage_2b?
+     //   ==>
+     //   var pkt := io.s;
+     //   && pkt.msg.ts >= ios[0].r.msg.ts + minD > t2a + 2*minD
+     //   );
+
+      // forall id | true
+        // ensures Progress2aProperty(progresses', id, s'.undeliveredPackets)
+      // {
+        // SelectiveProgress2aProperty(progresses', id, s'.undeliveredPackets);
+        // SelectiveProgress2aProperty(progresses, id, s.undeliveredPackets);
+      // }
+      assert Phase2UnacceptedLeaderInvariant(s', req_time, t2a, progresses');
+    }
+  }
+}
+
+lemma lemma_leader_notreceive_P2UnacceptedGoesToP2Unaccepted(s:TimestampedRslState, s':TimestampedRslState, j:int, req_time:Timestamp, t2a:Timestamp, progresses:map<NodeIdentity, Phase2Progress>)
+  returns (progresses':map<NodeIdentity,Phase2Progress>)
+
+  requires RslAssumption(s);
+  requires RslAssumption(s');
+  requires RslConsistency(s);
+  requires RslConsistency(s');
+  requires 0 <= j < |s.constants.config.replica_ids|;
+
+  requires j == 0;
+
+  requires s.t_environment.nextStep.LEnvStepHostIos?;
+  requires s.t_environment.nextStep.actor == s.constants.config.replica_ids[j];
+  requires s.t_environment.nextStep.nodeStep != RslStep(0);
+
+  requires TimestampedRslNextOneReplica(s, s', j, s.t_environment.nextStep.ios);
+
+  requires Phase2UnacceptedLeaderInvariant(s, req_time, t2a, progresses)
+  ensures Phase2UnacceptedLeaderInvariant(s', req_time, t2a, progresses')
+{
+  reveal_Progress2aProperty();
+  progresses' := progresses;
+}
+
+lemma lemma_leader_receive_P2UnacceptedGoesToP2(s:TimestampedRslState, s':TimestampedRslState, j:int, req_time:Timestamp, t2a:Timestamp, progresses:map<NodeIdentity, Phase2Progress>)
+  returns (progresses':map<NodeIdentity,Phase2Progress>)
+
+  requires RslAssumption(s);
+  requires RslAssumption(s');
+  requires RslConsistency(s);
+  requires RslConsistency(s');
+  requires 0 <= j < |s.constants.config.replica_ids|;
+
+  requires j == 0;
+
+  requires s.t_environment.nextStep.LEnvStepHostIos?;
+  requires s.t_environment.nextStep.actor == s.constants.config.replica_ids[j];
+  requires s.t_environment.nextStep.nodeStep != RslStep(0);
+
+  requires TimestampedRslNextOneReplica(s, s', j, s.t_environment.nextStep.ios);
+
+  requires Phase2UnacceptedLeaderInvariant(s, req_time, t2a, progresses)
+  ensures Phase2UnacceptedLeaderInvariant(s', req_time, t2a, progresses')
+{
+  reveal_Progress2aProperty();
+  progresses' := progresses;
 }
 
 }
